f-pure-v1: rename for better readability

f_cap_pure.v
@@ -18,8 +18,8 @@ Inductive typ       : Set   :=
   | typ_fvar        : var -> typ
   | typ_base        : typ
   | typ_eff         : typ
-  | typ_arrow_closed  : typ -> typ -> typ       (* effect closeded term abstraction *)
-  | typ_all_closed    : typ -> typ.             (* effect closeded type abstraction *)
+  | typ_stoic  : typ -> typ -> typ       (* effect closeded term abstraction *)
+  | typ_all    : typ -> typ.             (* effect closeded type abstraction *)
 
 (** Representation of pre-terms *)
 
@@ -39,8 +39,8 @@ Fixpoint open_tt_rec (K : nat) (U : typ) (T : typ) {struct T} : typ :=
   | typ_fvar X            => typ_fvar X
   | typ_base              => typ_base
   | typ_eff               => typ_eff
-  | typ_arrow_closed T1 T2  => typ_arrow_closed (open_tt_rec K U T1) (open_tt_rec K U T2)
-  | typ_all_closed T1       => typ_all_closed (open_tt_rec (S K) U T1)
+  | typ_stoic T1 T2       => typ_stoic (open_tt_rec K U T1) (open_tt_rec K U T2)
+  | typ_all T1            => typ_all (open_tt_rec (S K) U T1)
   end.
 
 Definition open_tt T U := open_tt_rec 0 U T.
@@ -67,7 +67,7 @@ Fixpoint open_ee_rec (k : nat) (f : trm) (e : trm) {struct e} : trm :=
   | trm_fvar x    => trm_fvar x
   | trm_abs V e1  => trm_abs V (open_ee_rec (S k) f e1)
   | trm_app e1 e2 => trm_app (open_ee_rec k f e1) (open_ee_rec k f e2)
-  | trm_tabs e1 => trm_tabs (open_ee_rec k f e1)
+  | trm_tabs e1   => trm_tabs (open_ee_rec k f e1)
   | trm_tapp e1 V => trm_tapp (open_ee_rec k f e1) V
   end.
 
@@ -86,13 +86,13 @@ Inductive type : typ -> Prop :=
       type (typ_fvar X)
   | type_base: type typ_base
   | type_eff: type typ_eff
-  | type_arrow_closed : forall T1 T2,
+  | type_stoic : forall T1 T2,
       type T1 ->
       type T2 ->
-      type (typ_arrow_closed T1 T2)
-  | type_all_closed : forall L T2,
+      type (typ_stoic T1 T2)
+  | type_all : forall L T2,
       (forall X, X \notin L -> type (T2 open_tt_var X)) ->
-      type (typ_all_closed T2).
+      type (typ_all T2).
 
 (** Terms as locally closeded pre-terms *)
 
@@ -122,12 +122,12 @@ Inductive term : trm -> Prop :=
  a typing assumption *)
 
 Inductive bind : Set :=
-  | bind_X : bind
-  | bind_x : typ -> bind.
+  | bind_tvar : bind
+  | bind_typ  : typ -> bind.
 
-Notation "[: X :]" := (X ~ bind_X)
+Notation "[: X :]" := (X ~ bind_tvar)
   (at level 23) : env_scope.
-Notation "x ~: T" := (x ~ bind_x T)
+Notation "x ~: T" := (x ~ bind_typ T)
   (at level 24, left associativity) : env_scope.
 
 Definition env := LibEnv.env bind.
@@ -138,16 +138,16 @@ Definition env := LibEnv.env bind.
 
 Inductive wft : env -> typ -> Prop :=
   | wft_var : forall E X,
-      binds X bind_X E ->
+      binds X bind_tvar E ->
       wft E (typ_fvar X)
-  | wft_arrow_closed : forall E T1 T2,
+  | wft_stoic : forall E T1 T2,
       wft E T1 ->
       wft E T2 ->
-      wft E (typ_arrow_closed T1 T2)
-  | wft_all_closed : forall L E T,
+      wft E (typ_stoic T1 T2)
+  | wft_all : forall L E T,
       (forall X, X \notin L ->
         wft (E & [: X :]) (T open_tt_var X)) ->
-      wft E (typ_all_closed T).
+      wft E (typ_all T).
 
 (** A environment E is well-formed if it contains no duplicate bindings
   and if each type in it is well-formed with respect to the environment
@@ -167,15 +167,15 @@ Fixpoint closed_typ(t: typ) := match t with
   | typ_fvar _          => true
   | typ_base            => true
   | typ_eff             => false
-  | typ_arrow_closed U V => true   (* pure lambda abstraction *)
-  | typ_all_closed T     => true   (* pure type abstraction *)
+  | typ_stoic U V       => true   (* effect-closed lambda abstraction *)
+  | typ_all T           => true   (* effect-closed type abstraction *)
   end.
 
 Fixpoint pure(E: env) := match E with
   | nil => nil
-  | cons (X, bind_X) E' => cons (X, bind_X) (pure E')
-  | cons (x, bind_x T) E' => if closed_typ T then
-                               cons (x, bind_x T) (pure E')
+  | cons (X, bind_tvar) E' => cons (X, bind_tvar) (pure E')
+  | cons (x, bind_typ T) E' => if closed_typ T then
+                               cons (x, bind_typ T) (pure E')
                              else
                                pure E'
     end.
@@ -184,24 +184,24 @@ Fixpoint pure(E: env) := match E with
 Inductive capsafe: typ -> Prop :=
  | capsafe_base: capsafe typ_base
  | capsafe_var: forall X, capsafe (typ_fvar X)
- | capsafe_eff_any: forall S T, type T -> caprod S -> capsafe (typ_arrow_closed S T)
- | capsafe_any_safe: forall S T, type S -> capsafe T -> capsafe (typ_arrow_closed S T)
- | capsafe_all: forall L T, type (typ_all_closed T) ->
+ | capsafe_eff_any: forall S T, type T -> caprod S -> capsafe (typ_stoic S T)
+ | capsafe_any_safe: forall S T, type S -> capsafe T -> capsafe (typ_stoic S T)
+ | capsafe_all: forall L T, type (typ_all T) ->
                           (forall X, X \notin L -> capsafe (T open_tt_var X)) ->
-                          capsafe (typ_all_closed T)
+                          capsafe (typ_all T)
 
 with caprod: typ -> Prop :=
  | caprod_eff: caprod typ_eff
- | caprod_safe_eff: forall S T, capsafe S -> caprod T -> caprod (typ_arrow_closed S T)
- | caprod_all: forall L T, type (typ_all_closed T) ->
+ | caprod_safe_eff: forall S T, capsafe S -> caprod T -> caprod (typ_stoic S T)
+ | caprod_all: forall L T, type (typ_all T) ->
                          (forall X, X \notin L -> caprod (T open_tt_var X)) ->
-                         caprod (typ_all_closed T).
+                         caprod (typ_all T).
 
 Inductive healthy: env -> Prop :=
   | healthy_empty: healthy empty
-  | healthy_push_x: forall x E T, capsafe T -> healthy E ->
+  | healthy_typ: forall x E T, capsafe T -> healthy E ->
                                   x # E -> healthy (E & x ~: T)
-  | healthy_push_X: forall X E, healthy E ->
+  | healthy_tvar: forall X E, healthy E ->
                                   X # E -> healthy (E & [: X :]).
 
 
@@ -210,25 +210,25 @@ Inductive healthy: env -> Prop :=
 Inductive typing : env -> trm -> typ -> Prop :=
   | typing_var : forall E x T,
       okt E ->
-      binds x (bind_x T) E ->
+      binds x (bind_typ T) E ->
       typing E (trm_fvar x) T
   | typing_abs_closed: forall L E V e1 T1,
       okt E ->
       (forall x, x \notin L ->
         typing ((pure E) & x ~: V) (e1 open_ee_var x) T1) ->
-      typing E (trm_abs V e1) (typ_arrow_closed V T1)
+      typing E (trm_abs V e1) (typ_stoic V T1)
   | typing_app : forall T1 E e1 e2 T2,
-      typing E e1 (typ_arrow_closed T1 T2) ->
+      typing E e1 (typ_stoic T1 T2) ->
       typing E e2 T1 ->
       typing E (trm_app e1 e2) T2
   | typing_tabs_closed : forall L E e1 T1,
       okt E ->
       (forall X, X \notin L ->
         typing ((pure E) & [: X :]) (e1 open_te_var X) (T1 open_tt_var X)) ->
-      typing E (trm_tabs e1) (typ_all_closed T1)
+      typing E (trm_tabs e1) (typ_all T1)
   | typing_tapp : forall T1 E e1 T,
       wft E T -> capsafe T ->
-      typing E e1 (typ_all_closed T1) ->
+      typing E e1 (typ_all T1) ->
       typing E (trm_tapp e1 T) (open_tt T1 T).
 
 (** Values *)
@@ -290,8 +290,8 @@ Fixpoint fv_tt (T : typ) {struct T} : vars :=
   | typ_base              => \{}
   | typ_eff               => \{}
   | typ_fvar X            => \{X}
-  | typ_arrow_closed T1 T2 => (fv_tt T1) \u (fv_tt T2)
-  | typ_all_closed T1      => (fv_tt T1)
+  | typ_stoic T1 T2 => (fv_tt T1) \u (fv_tt T2)
+  | typ_all T1      => (fv_tt T1)
   end.
 
 (** Computing free type variables in a term *)
@@ -326,8 +326,8 @@ Fixpoint subst_tt (Z : var) (U : typ) (T : typ) {struct T} : typ :=
   | typ_base              => typ_base
   | typ_eff               => typ_eff
   | typ_fvar X            => If X = Z then U else (typ_fvar X)
-  | typ_arrow_closed T1 T2 => typ_arrow_closed (subst_tt Z U T1) (subst_tt Z U T2)
-  | typ_all_closed T        => typ_all_closed (subst_tt Z U T)
+  | typ_stoic T1 T2 => typ_stoic (subst_tt Z U T1) (subst_tt Z U T2)
+  | typ_all T        => typ_all (subst_tt Z U T)
   end.
 
 (** Substitution for free type variables in terms. *)
@@ -358,8 +358,8 @@ Fixpoint subst_ee (z : var) (u : trm) (e : trm) {struct e} : trm :=
 
 Definition subst_tb (Z : var) (P : typ) (b : bind) : bind :=
   match b with
-  | bind_X => bind_X
-  | bind_x T => bind_x (subst_tt Z P T)
+  | bind_tvar => bind_tvar
+  | bind_typ T => bind_typ (subst_tt Z P T)
   end.
 
 (* ********************************************************************** *)
@@ -697,7 +697,7 @@ Lemma subst_tt_type : forall T Z P,
 Proof.
   induction 1; intros; simpl; auto.
   case_var*.
-  apply_fresh* type_all_closed as X. rewrite* subst_tt_open_tt_var.
+  apply_fresh* type_all as X. rewrite* subst_tt_open_tt_var.
 Qed.
 
 Lemma subst_te_term : forall e Z P,
@@ -744,7 +744,7 @@ Proof.
   apply wft_var. apply* binds_weaken.
   (* case arrow *)
   (* case: all *)
-  apply_fresh* wft_all_closed as Y. apply_ih_bind* H0.
+  apply_fresh* wft_all as Y. apply_ih_bind* H0.
 Qed.
 
 (** Through strengthening *)
@@ -761,7 +761,7 @@ Proof.
       subst. false.
       apply~ binds_concat_left.
   (* todo: binds_cases tactic *)
-  apply_fresh* wft_all_closed as Y. apply_ih_bind* H0.
+  apply_fresh* wft_all as Y. apply_ih_bind* H0.
 Qed.
 
 (** Through type substitution *)
@@ -778,13 +778,13 @@ Proof.
     destruct (binds_concat_inv H) as [?|[? ?]].
       apply wft_var.
        apply~ binds_concat_right.
-       replace bind_X with ((subst_tb Z P) bind_X) by reflexivity.
+       replace bind_tvar with ((subst_tb Z P) bind_tvar) by reflexivity.
        apply~ binds_map.
       destruct (binds_push_inv H1) as [[? ?]|[? ?]].
         subst. false~.
         applys wft_var. apply* binds_concat_left.
-  apply_fresh* wft_all_closed as Y.
-   unsimpl ((subst_tb Z P) bind_X).
+  apply_fresh* wft_all as Y.
+   unsimpl ((subst_tb Z P) bind_tvar).
    lets: wft_type.
    rewrite* subst_tt_open_tt_var.
    apply_ih_map_bind* H0.
@@ -794,7 +794,7 @@ Qed.
 
 Lemma wft_open : forall E U T,
   ok E ->
-  wft E (typ_all_closed T) ->
+  wft E (typ_all T) ->
   wft E U ->
   wft E (open_tt T U).
 Proof.
@@ -822,7 +822,7 @@ Hint Extern 1 (ok _) => apply ok_from_okt.
 (** Extraction from a typing assumption in a well-formed environments *)
 
 Lemma wft_from_env_has_typ : forall x U E,
-  okt E -> binds x (bind_x U) E -> wft E U.
+  okt E -> binds x (bind_typ U) E -> wft E U.
 Proof.
   induction E using env_ind; intros Ok B.
   false* binds_empty_inv.
@@ -872,7 +872,7 @@ Hint Resolve wft_subst_tb.
 (** Inversion lemma *)
 
 Lemma okt_push_inv : forall E X B,
-  okt (E & X ~ B) -> exists T, B = bind_X \/ B = bind_x T.
+  okt (E & X ~ B) -> exists T, B = bind_tvar \/ B = bind_typ T.
 Proof.
   introv O. inverts O.
     false* empty_push_inv.
@@ -880,7 +880,7 @@ Proof.
     lets (?&?&?): (eq_push_inv H). subst*.
 Qed.
 
-Lemma okt_push_X_inv : forall E X,
+Lemma okt_push_tvar_inv : forall E X,
   okt (E & [: X :]) -> okt E /\ X # E.
 Proof.
   introv O. inverts O.
@@ -889,7 +889,7 @@ Proof.
     lets (?&?&?): (eq_push_inv H). false.
 Qed.
 
-Lemma okt_push_x_inv : forall E x T,
+Lemma okt_push_typ_inv : forall E x T,
   okt (E & x ~: T) -> okt E /\ wft E T /\ x # E.
 Proof.
   introv O. inverts O.
@@ -898,11 +898,11 @@ Proof.
     lets (?&M&?): (eq_push_inv H). subst. inverts~ M.
 Qed.
 
-Lemma okt_push_x_type : forall E x T,
+Lemma okt_push_typ_type : forall E x T,
   okt (E & x ~: T) -> type T.
-Proof. intros. applys wft_type. forwards*: okt_push_x_inv. Qed.
+Proof. intros. applys wft_type. forwards*: okt_push_typ_inv. Qed.
 
-Hint Immediate okt_push_x_type.
+Hint Immediate okt_push_typ_type.
 
 (** Through strengthening *)
 
@@ -911,14 +911,14 @@ Lemma okt_strengthen : forall x T (E F:env),
   okt (E & F).
 Proof.
  introv O. induction F using env_ind.
-  rewrite concat_empty_r in *. lets*: (okt_push_x_inv O).
+  rewrite concat_empty_r in *. lets*: (okt_push_typ_inv O).
   rewrite concat_assoc in *.
    lets (U&[?|?]): okt_push_inv O; subst.
-      applys~ okt_X. apply IHF. applys* okt_push_X_inv.
+      applys~ okt_X. apply IHF. applys* okt_push_tvar_inv.
       apply ok_from_okt in O.
       lets (? & H): (ok_push_inv O). eauto.
 
-      applys~ okt_typ. apply IHF. applys* okt_push_x_inv.
+      applys~ okt_typ. apply IHF. applys* okt_push_typ_inv.
       applys* wft_strengthen.
       apply ok_from_okt in O.
       lets (? & H): (ok_push_inv O). eauto.
@@ -929,8 +929,8 @@ Lemma okt_weaken : forall E F,
 Proof.
   induction F using env_ind; rew_env_concat; introv Okt. auto.
   lets(T & [H | H]): (okt_push_inv Okt); subst.
-  apply IHF. lets*: okt_push_X_inv Okt.
-  apply IHF. lets*: okt_push_x_inv Okt.
+  apply IHF. lets*: okt_push_tvar_inv Okt.
+  apply IHF. lets*: okt_push_typ_inv Okt.
 Qed.
 
 (** Through type substitution *)
@@ -942,11 +942,11 @@ Lemma okt_subst_tb : forall Z P (E F:env),
 Proof.
  introv O W. induction F using env_ind.
   rewrite map_empty. rewrite concat_empty_r in *.
-   lets*: (okt_push_X_inv O).
+   lets*: (okt_push_tvar_inv O).
   rewrite map_push. rewrite concat_assoc in *.
    lets (U&[?|?]): okt_push_inv O; subst.
-     lets*: (okt_push_X_inv O).
-     lets*: (okt_push_x_inv O).
+     lets*: (okt_push_tvar_inv O).
+     lets*: (okt_push_typ_inv O).
       applys~ okt_typ; lets*: H.
 Qed.
 
@@ -1000,7 +1000,7 @@ Proof.
     pick_fresh y. specializes H1 y. destructs~ H1.
     apply_fresh* term_abs as y.
       pick_fresh y. specializes H1 y. destructs~ H1.
-        forwards*: okt_push_x_inv.
+        forwards*: okt_push_typ_inv.
       specializes H1 y. destructs~ H1.
   splits*.
   splits*.
@@ -1091,7 +1091,7 @@ Proof. intros. induction E.
       rewrite <- concat_empty_r. apply binds_weaken; rewrite* concat_empty_r.
 Qed.
 
-Lemma pure_binds_reverse: forall E x, binds x bind_X E -> binds x bind_X (pure E).
+Lemma pure_binds_reverse: forall E x, binds x bind_tvar E -> binds x bind_tvar (pure E).
 Proof. intros. induction E.
   simpl in *. autos.
   destruct a. destruct b.
@@ -1103,17 +1103,17 @@ Proof. intros. induction E.
 Qed.
 
 Lemma pure_binds_in: forall E x T, closed_typ T = true ->
-   binds x (bind_x T) E -> binds x (bind_x T) (pure E).
+   binds x (bind_typ T) E -> binds x (bind_typ T) (pure E).
 Proof. intros. induction E.
   (* nil *)
   rewrite <- empty_def in H0. destruct(binds_empty_inv H0).
   (* x::xs *)
   destruct a. destruct b.
-    (* bind_X *)
+    (* bind_tvar *)
     simpl. rewrite cons_to_push in *. destruct (binds_push_inv H0).
     destruct H1. inversion H2.
     destruct H1. apply* binds_push_neq.
-    (* bind_x *)
+    (* bind_typ *)
     simpls. rewrite cons_to_push in *. destruct (binds_push_inv H0).
     destruct H1. inversions H2. rewrite* H.
     destruct H1. destruct* (closed_typ t).
@@ -1122,8 +1122,8 @@ Qed.
 Lemma pure_wft: forall E V, ok E -> wft (pure E) V -> wft E V.
 Proof. intros. remember (pure E) as G. gen E. induction H0; intros; subst.
   apply wft_var. apply* pure_binds.
-  apply* wft_arrow_closed.
-  apply_fresh* wft_all_closed as Y. apply* H0. repeat(rewrite <- cons_to_push). autos.
+  apply* wft_stoic.
+  apply_fresh* wft_all as Y. apply* H0. repeat(rewrite <- cons_to_push). autos.
 Qed.
 
 Lemma pure_wft_weaken: forall E F G V,
@@ -1134,8 +1134,8 @@ Proof. intros. inductions H0; intros; subst.
     apply binds_concat_left; autos. apply* binds_concat_right. apply* pure_binds.
       lets*: ok_concat_inv_r (ok_concat_inv_l H).
     apply binds_concat_right. auto.
-  apply* wft_arrow_closed.
-  apply_fresh* wft_all_closed as Y.
+  apply* wft_stoic.
+  apply_fresh* wft_all as Y.
     assert (HI: ok (E & F & (G & [: Y :]))).
       rewrite concat_assoc. apply* ok_push.
     forwards~ HII: (H0 Y). apply HI.  rewrite* concat_assoc.
@@ -1145,8 +1145,8 @@ Qed.
 Lemma pure_wft_reverse: forall E V, wft E V -> wft (pure E) V.
 Proof. intros. induction H.
   apply wft_var. apply* pure_binds_reverse.
-  apply* wft_arrow_closed.
-  apply_fresh* wft_all_closed as Y. forwards~ HI: (H0 Y).
+  apply* wft_stoic.
+  apply_fresh* wft_all as Y. forwards~ HI: (H0 Y).
     rewrite pure_dist in HI. rewrite single_def in *. autos.
 Qed.
 
@@ -1178,9 +1178,9 @@ Lemma pure_okt : forall E,
   okt E -> okt (pure E).
 Proof. intros. induction* E.
   destruct a. destruct b; simpl; rewrite cons_to_push in *.
-  apply okt_X. apply IHE. lets*: okt_push_X_inv H.
-  unfolds. lets(_ & HI): okt_push_X_inv H. autos* (pure_dom_subset E).
-  destructs (okt_push_x_inv H). destruct* (closed_typ t).
+  apply okt_X. apply IHE. lets*: okt_push_tvar_inv H.
+  unfolds. lets(_ & HI): okt_push_tvar_inv H. autos* (pure_dom_subset E).
+  destructs (okt_push_typ_inv H). destruct* (closed_typ t).
     apply okt_typ. apply* IHE. apply* pure_wft_reverse.
     lets: pure_dom_subset E. unfolds subset.
     unfolds notin. autos.
@@ -1263,7 +1263,7 @@ Qed.
 Lemma typing_wft: forall E e T, typing E e T -> wft E T.
 Proof.
   intros. induction H. applys~ wft_from_env_has_typ x.
-  apply wft_arrow_closed. pick_fresh x. forwards~: (H0 x).
+  apply wft_stoic. pick_fresh x. forwards~: (H0 x).
     lets(H3 & _): (typing_regular H2). lets*: wft_from_okt_typ H3.
     apply* pure_wft.
 
@@ -1271,7 +1271,7 @@ Proof.
     rewrite <- (@concat_empty_r bind (x ~: V) ) in H2. rewrite concat_assoc in H2.
     lets: wft_strengthen H2. rewrite concat_empty_r in H3. apply* pure_wft.
   inverts* IHtyping1.
-  let L := gather_vars in (apply* (@wft_all_closed L)). intros.
+  let L := gather_vars in (apply* (@wft_all L)). intros.
     forwards~: (H1 X). rewrite <- (@concat_empty_l bind E).
     apply pure_wft_weaken; rewrite* concat_empty_l.
   apply* wft_open.
@@ -1338,10 +1338,10 @@ Lemma capsafe_subst_tt: forall T,
         ); intros; simpls; eauto.
   case_if*.
   let L' := gather_vars in apply capsafe_all with L'; auto.
-    unsimpl (subst_tt Z P (typ_all_closed T)). auto.
+    unsimpl (subst_tt Z P (typ_all T)). auto.
     intros. rewrite* subst_tt_open_tt_var.
   let L' := gather_vars in apply caprod_all with L'; auto.
-    unsimpl (subst_tt Z P (typ_all_closed T)). auto.
+    unsimpl (subst_tt Z P (typ_all T)). auto.
     intros. rewrite* subst_tt_open_tt_var.
 Qed.
 
@@ -1353,10 +1353,10 @@ Lemma caprod_subst_tt: forall T,
         ); intros; simpls; eauto.
   case_if*.
   let L' := gather_vars in apply capsafe_all with L'; auto.
-    unsimpl (subst_tt Z P (typ_all_closed T)). auto.
+    unsimpl (subst_tt Z P (typ_all T)). auto.
     intros. rewrite* subst_tt_open_tt_var.
   let L' := gather_vars in apply caprod_all with L'; auto.
-    unsimpl (subst_tt Z P (typ_all_closed T)). auto.
+    unsimpl (subst_tt Z P (typ_all T)). auto.
     intros. rewrite* subst_tt_open_tt_var.
 Qed.
 
@@ -1384,10 +1384,10 @@ Qed.
 Lemma capsafe_caprod_classic: forall T, type T -> capsafe T \/ caprod T.
 Proof. intros T Ht. inductions Ht; iauto.
   pick_fresh X. forwards~ : H0 X. destruct H1.
-  left. apply capsafe_all with (L \u fv_tt T2). apply* type_all_closed.
+  left. apply capsafe_all with (L \u fv_tt T2). apply* type_all.
     intros. forwards~ : capsafe_subst_tt H1 X (typ_fvar X0).
     rewrite* <- (@subst_tt_intro X) in H3.
-  right. apply caprod_all with L. apply* type_all_closed.
+  right. apply caprod_all with L. apply* type_all.
     intros. forwards~ : caprod_subst_tt H1 X (typ_fvar X0).
     rewrite* <- (@subst_tt_intro X) in H3.
 Qed.
@@ -1409,7 +1409,7 @@ Proof. intros. inductions H.
 Qed.
 
 Lemma healthy_env_capsafe : forall E S x, healthy E ->
-   binds x (bind_x S) E ->  capsafe S.
+   binds x (bind_typ S) E ->  capsafe S.
 Proof. introv H Hb. inductions H.
   false* binds_empty_inv.
   destruct (binds_push_inv Hb).
@@ -1599,14 +1599,14 @@ Proof.
   apply_fresh* typing_abs_closed as y.
     repeat(rewrite pure_dist in *). rewrite pure_single_tvar in *.
     rewrite* subst_te_open_ee_var. rewrite* pure_map.
-    unsimpl (subst_tb Z P (bind_x V)). rewrite <- concat_assoc. rewrite <- map_push.
+    unsimpl (subst_tb Z P (bind_typ V)). rewrite <- concat_assoc. rewrite <- map_push.
     apply* H1. rewrite* concat_assoc. apply* pure_wft_reverse.
   apply* typing_app.
   apply_fresh* typing_tabs_closed as Y.
     repeat(rewrite pure_dist in *). rewrite pure_single_tvar in *.
     rewrite* subst_te_open_te_var; eauto using wft_type.
     rewrite* subst_tt_open_tt_var; eauto using wft_type.
-    rewrite* pure_map. unsimpl (subst_tb Z P bind_X).
+    rewrite* pure_map. unsimpl (subst_tb Z P bind_tvar).
     rewrite <- concat_assoc. rewrite <- map_push.
     apply* H1. rewrite* concat_assoc. apply* pure_wft_reverse.
   rewrite* subst_tt_open_tt.
@@ -1651,21 +1651,21 @@ Qed.
 (** Canonical Forms (14) *)
 
 Lemma canonical_form_abs : forall t U1 U2,
-  value t -> typing empty t (typ_arrow_closed U1 U2) ->
+  value t -> typing empty t (typ_stoic U1 U2) ->
   exists V, exists e1, t = trm_abs V e1.
 Proof.
   introv Val Typ. gen_eq E: (@empty bind).
-  gen_eq T: (typ_arrow_closed U1 U2). gen U1 U2.
+  gen_eq T: (typ_stoic U1 U2). gen U1 U2.
   induction Typ; introv EQT EQE;
    try solve [ inversion Val | inversion EQT | eauto ].
 Qed.
 
 Lemma canonical_form_tabs : forall t U1,
-  value t -> typing empty t (typ_all_closed U1) ->
+  value t -> typing empty t (typ_all U1) ->
   exists e1, t = trm_tabs e1.
 Proof.
   introv Val Typ. gen_eq E: (@empty bind).
-  gen_eq T: (typ_all_closed U1). gen U1.
+  gen_eq T: (typ_all U1). gen U1.
   induction Typ; introv EQT EQE;
    try solve [ inversion Val | inversion EQT | eauto ].
 Qed.
@@ -1706,13 +1706,13 @@ Proof. intros. inductions H0.
     assert (HI: type V) by destruct* (typing_regular H3).
     destruct (capsafe_decidable HI).
       apply* capsafe_any_safe. apply* (H2 x). rewrite* (healthy_env_closed H).
-      apply* healthy_push_x. lets*: not_capsafe_caprod H4.
+      apply* healthy_typ. lets*: not_capsafe_caprod H4.
       apply* capsafe_eff_any. autos* wft_type typing_wft.
   forwards~ : IHtyping1 H. forwards~ : IHtyping2 H. inversions* H0.
     lets*: capsafe_not_caprod T1.
-  assert (typing E (trm_tabs e1) (typ_all_closed T1)) by apply* typing_tabs_closed.
+  assert (typing E (trm_tabs e1) (typ_all T1)) by apply* typing_tabs_closed.
     let L' := gather_vars in apply capsafe_all with L'; autos* wft_type typing_wft.
-    intros. apply* H2. rewrite* (healthy_env_closed H). apply* healthy_push_X.
+    intros. apply* H2. rewrite* (healthy_env_closed H). apply* healthy_tvar.
   lets: IHtyping H. inversions H3. pick_fresh X. forwards~ : H6 X.
     forwards~ : capsafe_subst_tt H3 X T.
     rewrite* <- (@subst_tt_intro X) in H4.
